backends/lean/Aeneas/Std/Scalar/OverflowingOps.lean
@@ -12,11 +12,11 @@ open ScalarElab
 -- TODO: we should redefine this, in particular so that it doesn't live in the `Result` monad
 
 def UScalar.overflowing_add {ty} (x y : UScalar ty) : UScalar ty × Bool :=
-  (UScalar.ofBitVec ty (BitVec.ofNat ty.numBits (x.val + y.val)), 2^ty.numBits ≤ x.val + y.val)
+  (UScalar.ofBitVec ty (BitVec.ofNat ty.numBits (x.toNat + y.toNat)), 2^ty.numBits ≤ x.toNat + y.toNat)
 
 def IScalar.overflowing_add (ty : IScalarTy) (x y : IScalar ty) : IScalar ty × Bool :=
-  (IScalar.ofBitVec ty (BitVec.ofInt ty.numBits (x.val + y.val)),
-     ¬ (-2^(ty.numBits -1) ≤ x.val + y.val ∧ x.val + y.val < 2^(ty.numBits-1)))
+  (IScalar.ofBitVec ty (BitVec.ofInt ty.numBits (x.toInt + y.toInt)),
+     ¬ (-2^(ty.numBits -1) ≤ x.toInt + y.toInt ∧ x.toInt + y.toInt < 2^(ty.numBits-1)))
 
 /- [core::num::{u8}::overflowing_add] -/
 uscalar def core.num.«%S».overflowing_add := @UScalar.overflowing_add .«%S»
@@ -28,28 +28,28 @@ attribute [-simp] Bool.exists_bool
 
 theorem UScalar.overflowing_add_eq {ty} (x y : UScalar ty) :
   let z := overflowing_add x y
-  if x.val + y.val > UScalar.max ty then
-    z.fst.val + UScalar.size ty = x.val + y.val ∧
+  if x.toNat + y.toNat > UScalar.max ty then
+    z.fst.toNat + UScalar.size ty = x.toNat + y.toNat ∧
     z.snd = true
   else
-    z.fst.val = x.val + y.val ∧
+    z.fst.toNat = x.toNat + y.toNat ∧
     z.snd = false
   := by
   have hx := x.hBounds
   have hy := y.hBounds
   have hN : 0 < 2 ^ ty.numBits := by simp
-  simp only [overflowing_add, UScalar.ofBitVec_val, BitVec.toNat_ofNat,
+  simp only [overflowing_add, UScalar.ofBitVec_toNat, BitVec.toNat_ofNat,
              UScalar.max, UScalar.size]
   split <;> rename_i hLt
   · refine ⟨?_, ?_⟩
     · have : (x.toNat + y.toNat) % 2^ty.numBits =
-             (x.bv.toNat + y.bv.toNat - 2^ty.numBits) % 2^ty.numBits := by
+             (x.toBitVec.toNat + y.toBitVec.toNat - 2^ty.numBits) % 2^ty.numBits := by
         rw [Nat.mod_eq_sub_mod]
         · cases ty <;> grind
         · grind
       rw [this]; clear this
 
-      have := @Nat.mod_eq_of_lt (x.bv.toNat + y.bv.toNat - 2^ty.numBits) (2^ty.numBits) (by omega)
+      have := @Nat.mod_eq_of_lt (x.toBitVec.toNat + y.toBitVec.toNat - 2^ty.numBits) (2^ty.numBits) (by omega)
       rw [this]; clear this
       scalar_tac
     · simp only [decide_eq_true_eq]; omega
@@ -60,8 +60,8 @@ theorem UScalar.overflowing_add_eq {ty} (x y : UScalar ty) :
 uscalar @[step_pure overflowing_add x y]
 theorem core.num.«%S».overflowing_add_eq (x y : «%S») :
   let z := overflowing_add x y
-  if x.val + y.val > UScalar.max .«%S» then z.fst.val + UScalar.size .«%S» = x.val + y.val ∧ z.snd = true
-  else z.fst.val = x.val + y.val ∧ z.snd = false
+  if x.toNat + y.toNat > UScalar.max .«%S» then z.fst.toNat + UScalar.size .«%S» = x.toNat + y.toNat ∧ z.snd = true
+  else z.fst.toNat = x.toNat + y.toNat ∧ z.snd = false
   := UScalar.overflowing_add_eq x y
 
 end Aeneas.Std
