backends/lean/Aeneas/Std/Scalar/WrappingOps/Mul.lean
@@ -9,9 +9,9 @@ open Result Error ScalarElab
 # Wrapping Mul
 -/
 
-def UScalar.wrapping_mul {ty} (x y : UScalar ty) : UScalar ty := UScalar.ofBitVec ty (x.bv * y.bv)
+def UScalar.wrapping_mul {ty} (x y : UScalar ty) : UScalar ty := UScalar.ofBitVec ty (x.toBitVec * y.toBitVec)
 
-def IScalar.wrapping_mul {ty} (x y : IScalar ty) : IScalar ty := IScalar.ofBitVec ty (x.bv * y.bv)
+def IScalar.wrapping_mul {ty} (x y : IScalar ty) : IScalar ty := IScalar.ofBitVec ty (x.toBitVec * y.toBitVec)
 
 uscalar @[step_pure_def]
 def «%S».wrapping_mul (x y : «%S») : «%S» := @UScalar.wrapping_mul UScalarTy.«%S» x y
@@ -27,52 +27,52 @@ def core.num.«%S».wrapping_mul : «%S» → «%S» → «%S» := @UScalar.wrap
 iscalar @[step_pure_def]
 def core.num.«%S».wrapping_mul : «%S» → «%S» → «%S»  := @IScalar.wrapping_mul IScalarTy.«%S»
 
-@[simp, bvify, grind =, agrind =] theorem UScalar.wrapping_mul_bv_eq {ty} (x y : UScalar ty) :
-  (wrapping_mul x y).bv = x.bv * y.bv := by
-  simp only [wrapping_mul, UScalar.ofBitVec_bv]
+@[simp, bvify, grind =, agrind =] theorem UScalar.wrapping_mul_toBitVec_eq {ty} (x y : UScalar ty) :
+  (wrapping_mul x y).toBitVec = x.toBitVec * y.toBitVec := by
+  simp only [wrapping_mul, UScalar.ofBitVec_toBitVec]
 
-uscalar @[simp, bvify, grind =, agrind =] theorem «%S».wrapping_mul_bv_eq (x y : «%S») :
-  («%S».wrapping_mul x y).bv = x.bv * y.bv :=
-  UScalar.wrapping_mul_bv_eq x y
+uscalar @[simp, bvify, grind =, agrind =] theorem «%S».wrapping_mul_toBitVec_eq (x y : «%S») :
+  («%S».wrapping_mul x y).toBitVec = x.toBitVec * y.toBitVec :=
+  UScalar.wrapping_mul_toBitVec_eq x y
 
-uscalar @[simp, bvify, grind =, agrind =] theorem core.num.«%S».wrapping_mul_bv_eq (x y : «%S») :
-  (core.num.«%S».wrapping_mul x y).bv = x.bv * y.bv :=
-  UScalar.wrapping_mul_bv_eq x y
+uscalar @[simp, bvify, grind =, agrind =] theorem core.num.«%S».wrapping_mul_toBitVec_eq (x y : «%S») :
+  (core.num.«%S».wrapping_mul x y).toBitVec = x.toBitVec * y.toBitVec :=
+  UScalar.wrapping_mul_toBitVec_eq x y
 
-@[simp, bvify, grind =, agrind =] theorem IScalar.wrapping_mul_bv_eq {ty} (x y : IScalar ty) :
-  (wrapping_mul x y).bv = x.bv * y.bv := by
-  simp only [wrapping_mul, IScalar.ofBitVec_bv]
+@[simp, bvify, grind =, agrind =] theorem IScalar.wrapping_mul_toBitVec_eq {ty} (x y : IScalar ty) :
+  (wrapping_mul x y).toBitVec = x.toBitVec * y.toBitVec := by
+  simp only [wrapping_mul, IScalar.ofBitVec_toBitVec]
 
-iscalar @[simp, bvify, grind =, agrind =] theorem «%S».wrapping_mul_bv_eq (x y : «%S») :
-  («%S».wrapping_mul x y).bv = x.bv * y.bv :=
-  IScalar.wrapping_mul_bv_eq x y
+iscalar @[simp, bvify, grind =, agrind =] theorem «%S».wrapping_mul_toBitVec_eq (x y : «%S») :
+  («%S».wrapping_mul x y).toBitVec = x.toBitVec * y.toBitVec :=
+  IScalar.wrapping_mul_toBitVec_eq x y
 
-iscalar @[simp, bvify, grind =, agrind =] theorem core.num.«%S».wrapping_mul_bv_eq (x y : «%S») :
-  (core.num.«%S».wrapping_mul x y).bv = x.bv * y.bv :=
-  IScalar.wrapping_mul_bv_eq x y
+iscalar @[simp, bvify, grind =, agrind =] theorem core.num.«%S».wrapping_mul_toBitVec_eq (x y : «%S») :
+  (core.num.«%S».wrapping_mul x y).toBitVec = x.toBitVec * y.toBitVec :=
+  IScalar.wrapping_mul_toBitVec_eq x y
 
-@[simp] theorem UScalar.wrapping_mul_val_eq {ty} (x y : UScalar ty) :
-  (wrapping_mul x y).val = (x.val * y.val) % (UScalar.size ty) := by
-  simp only [wrapping_mul, UScalar.ofBitVec_val, BitVec.toNat_mul, bv_toNat, size]
+@[simp] theorem UScalar.wrapping_mul_toNat_eq {ty} (x y : UScalar ty) :
+  (wrapping_mul x y).toNat = (x.toNat * y.toNat) % (UScalar.size ty) := by
+  simp only [wrapping_mul, UScalar.ofBitVec_toNat, BitVec.toNat_mul, toBitVec_toNat, size]
 
-uscalar @[simp, grind =, agrind =] theorem «%S».wrapping_mul_val_eq (x y : «%S») :
-  («%S».wrapping_mul x y).val = (x.val * y.val) % (UScalar.size .«%S») :=
-  UScalar.wrapping_mul_val_eq x y
+uscalar @[simp, grind =, agrind =] theorem «%S».wrapping_mul_toNat_eq (x y : «%S») :
+  («%S».wrapping_mul x y).toNat = (x.toNat * y.toNat) % (UScalar.size .«%S») :=
+  UScalar.wrapping_mul_toNat_eq x y
 
-uscalar @[simp, grind =, agrind =] theorem core.num.«%S».wrapping_mul_val_eq (x y : «%S») :
-  (core.num.«%S».wrapping_mul x y).val = (x.val * y.val) % (UScalar.size .«%S») :=
-  UScalar.wrapping_mul_val_eq x y
+uscalar @[simp, grind =, agrind =] theorem core.num.«%S».wrapping_mul_toNat_eq (x y : «%S») :
+  (core.num.«%S».wrapping_mul x y).toNat = (x.toNat * y.toNat) % (UScalar.size .«%S») :=
+  UScalar.wrapping_mul_toNat_eq x y
 
-@[simp] theorem IScalar.wrapping_mul_val_eq {ty} (x y : IScalar ty) :
-  (wrapping_mul x y).val = Int.bmod (x.val * y.val) (2^ty.numBits) := by
-  simp only [wrapping_mul, IScalar.ofBitVec_val, BitVec.toInt_mul, bv_toInt_eq]
+@[simp] theorem IScalar.wrapping_mul_toInt_eq {ty} (x y : IScalar ty) :
+  (wrapping_mul x y).toInt = Int.bmod (x.toInt * y.toInt) (2^ty.numBits) := by
+  simp only [wrapping_mul, IScalar.ofBitVec_toInt, BitVec.toInt_mul, toBitVec_toInt]
 
-iscalar @[simp, grind =, agrind =] theorem «%S».wrapping_mul_val_eq (x y : «%S») :
-  («%S».wrapping_mul x y).val = Int.bmod (x.val * y.val) (2^ %BitWidth) :=
-  IScalar.wrapping_mul_val_eq x y
+iscalar @[simp, grind =, agrind =] theorem «%S».wrapping_mul_toInt_eq (x y : «%S») :
+  («%S».wrapping_mul x y).toInt = Int.bmod (x.toInt * y.toInt) (2^ %BitWidth) :=
+  IScalar.wrapping_mul_toInt_eq x y
 
-iscalar @[simp, grind =, agrind =] theorem core.num.«%S».wrapping_mul_val_eq (x y : «%S») :
-  (core.num.«%S».wrapping_mul x y).val = Int.bmod (x.val * y.val) (2^ %BitWidth) :=
-  IScalar.wrapping_mul_val_eq x y
+iscalar @[simp, grind =, agrind =] theorem core.num.«%S».wrapping_mul_toInt_eq (x y : «%S») :
+  (core.num.«%S».wrapping_mul x y).toInt = Int.bmod (x.toInt * y.toInt) (2^ %BitWidth) :=
+  IScalar.wrapping_mul_toInt_eq x y
 
 end Aeneas.Std
