backends/lean/Aeneas/Std/Scalar/SaturatingOps.lean
@@ -13,7 +13,7 @@ open Result Error ScalarElab
 Saturating add: unsigned
 -/
 def UScalar.saturating_add {ty : UScalarTy} (x y : UScalar ty) : UScalar ty :=
-  UScalar.ofBitVec ty (BitVec.ofNat ty.numBits (Min.min (UScalar.max ty) (x.val + y.val)))
+  UScalar.ofBitVec ty (BitVec.ofNat ty.numBits (Min.min (UScalar.max ty) (x.toNat + y.toNat)))
 
 /- [core::num::{u8}::saturating_add] -/
 uscalar def core.num.«%S».saturating_add := @UScalar.saturating_add UScalarTy.«%S»
@@ -22,7 +22,7 @@ uscalar def core.num.«%S».saturating_add := @UScalar.saturating_add UScalarTy.
 Saturating add: signed
 -/
 def IScalar.saturating_add {ty : IScalarTy} (x y : IScalar ty) : IScalar ty :=
-  IScalar.ofBitVec ty (BitVec.ofInt ty.numBits (Max.max (IScalar.min ty) (Min.min (IScalar.max ty) (x.val + y.val))))
+  IScalar.ofBitVec ty (BitVec.ofInt ty.numBits (Max.max (IScalar.min ty) (Min.min (IScalar.max ty) (x.toInt + y.toInt))))
 
 /- [core::num::{i8}::saturating_add] -/
 iscalar def core.num.«%S».saturating_add := @IScalar.saturating_add IScalarTy.«%S»
@@ -31,7 +31,7 @@ iscalar def core.num.«%S».saturating_add := @IScalar.saturating_add IScalarTy.
 Saturating sub: unsigned
 -/
 def UScalar.saturating_sub {ty : UScalarTy} (x y : UScalar ty) : UScalar ty :=
-  UScalar.ofBitVec ty (BitVec.ofNat ty.numBits (Max.max 0 (x.val - y.val)))
+  UScalar.ofBitVec ty (BitVec.ofNat ty.numBits (Max.max 0 (x.toNat - y.toNat)))
 
 /- [core::num::{u8}::saturating_sub] -/
 uscalar def core.num.«%S».saturating_sub := @UScalar.saturating_sub UScalarTy.«%S»
@@ -40,7 +40,7 @@ uscalar def core.num.«%S».saturating_sub := @UScalar.saturating_sub UScalarTy.
 Saturating sub: signed
 -/
 def IScalar.saturating_sub {ty : IScalarTy} (x y : IScalar ty) : IScalar ty :=
-  IScalar.ofBitVec ty (BitVec.ofInt ty.numBits (Max.max (IScalar.min ty) (Min.min (IScalar.max ty) (x.val - y.val))))
+  IScalar.ofBitVec ty (BitVec.ofInt ty.numBits (Max.max (IScalar.min ty) (Min.min (IScalar.max ty) (x.toInt - y.toInt))))
 
 /- [core::num::{i8}::saturating_sub] -/
 iscalar def core.num.«%S».saturating_sub := @IScalar.saturating_sub IScalarTy.«%S»
